src/asn1/ASN1.Spec.Tag.fst
@@ -6,15 +6,15 @@ open LowParse.Spec.Int
 
 open ASN1.Base
 
-(* Tag parser primitive *)
-
+/// Generic
+///
 let filter_asn1_tag
   (b: byte)
 : Ghost bool
   (requires True)
-  (ensures fun r -> r == (b = 0x01uy || b = 0x04uy || b = 0x05uy))
+  (ensures fun r -> r == (b = 0x01uy || b = 0x04uy || b = 0x05uy || b = 0x30uy))
 = match b with
-  | 0x01uy | 0x04uy | 0x05uy -> true
+  | 0x01uy | 0x04uy | 0x05uy | 0x30uy-> true
   | _ -> false
 
 let synth_asn1_tag
@@ -25,11 +25,13 @@ let synth_asn1_tag
     a == (match b with
           | 0x01uy -> BOOLEAN
           | 0x04uy -> OCTET_STRING
-          | 0x05uy -> NULL))
+          | 0x05uy -> NULL
+          | 0x30uy -> SEQUENCE))
 = match b with
   | 0x01uy -> BOOLEAN
   | 0x04uy -> OCTET_STRING
   | 0x05uy -> NULL
+  | 0x30uy -> SEQUENCE
 
 let synth_asn1_tag_inverse
   (a: asn1_type)
@@ -43,7 +45,7 @@ let synth_asn1_tag_inverse
   | OCTET_STRING -> 0x04uy
   | NULL         -> 0x05uy
   // | OID          -> 0x06uy
-  // | SEQUENCE     -> 0x30uy
+  | SEQUENCE     -> 0x30uy
 
 let parse_asn1_tag
 : parser parse_asn1_tag_kind asn1_type
@@ -105,3 +107,100 @@ let serialize_asn1_tag_unfold
   (* g1 *) (synth_asn1_tag_inverse)
   (* prf*) ()
   (* in *) (a)
+
+/// Specialied
+///
+let filter_the_asn1_tag
+  (a: asn1_type)
+  (b: byte)
+: Ghost bool
+  (requires True)
+  (ensures fun r -> (r <==> filter_asn1_tag b /\ synth_asn1_tag b == a))
+= match a, b with
+  | BOOLEAN     , 0x01uy
+  | OCTET_STRING, 0x04uy
+  | NULL        , 0x05uy
+  | SEQUENCE    , 0x30uy -> true
+  | _ -> false
+
+let synth_the_asn1_tag
+  (a: asn1_type)
+  (b: parse_filter_refine (filter_the_asn1_tag a))
+: Ghost (the_asn1_type a)
+  (requires True)
+  (ensures fun a' -> (a' == synth_asn1_tag b))
+= a
+
+let synth_the_asn1_tag_inverse
+  (a: asn1_type)
+  (a': the_asn1_type a)
+: Ghost (parse_filter_refine (filter_the_asn1_tag a))
+  (requires True)
+  (ensures fun b -> (b == synth_asn1_tag_inverse a'))
+= synth_asn1_tag_inverse a'
+
+let parse_the_asn1_tag
+  (a: asn1_type)
+: parser parse_asn1_tag_kind (the_asn1_type a)
+= parse_u8
+  `parse_filter`
+  filter_the_asn1_tag a
+  `parse_synth`
+  synth_the_asn1_tag a
+
+let parse_the_asn1_tag_unfold
+  (a: asn1_type)
+  (input: bytes)
+: Lemma (
+  parse (parse_the_asn1_tag a) input ==
+ (match parse parse_u8 input with
+  | Some (x, consumed) -> if filter_the_asn1_tag a x then
+                          ( Some (synth_the_asn1_tag a x, consumed) )
+                          else
+                          ( None )
+  | None -> None))
+= parser_kind_prop_equiv parse_asn1_tag_kind (parse_the_asn1_tag a);
+  parse_filter_eq
+  (* p  *) (parse_u8)
+  (* f  *) (filter_the_asn1_tag a)
+  (* in *) (input);
+  parse_synth_eq
+  (* p1 *) (parse_u8
+            `parse_filter`
+            filter_the_asn1_tag a)
+  (* f2 *) (synth_the_asn1_tag a)
+  (* in *) (input)
+
+let serialize_the_asn1_tag
+  (a: asn1_type)
+: serializer (parse_the_asn1_tag a)
+= serialize_synth
+  (* p1 *) (parse_u8
+            `parse_filter`
+            filter_the_asn1_tag a)
+  (* f2 *) (synth_the_asn1_tag a)
+  (* s1 *) (serialize_u8
+            `serialize_filter`
+            filter_the_asn1_tag a)
+  (* g1 *) (synth_the_asn1_tag_inverse a)
+  (* prf*) ()
+
+let serialize_the_asn1_tag_unfold
+  (a: asn1_type)
+  (a': the_asn1_type a)
+: Lemma (
+  serialize (serialize_the_asn1_tag a) a'
+  `Seq.equal`
+  serialize serialize_u8 (synth_the_asn1_tag_inverse a a'))
+= serialize_synth_eq
+  (* p1 *) (parse_u8
+            `parse_filter`
+            filter_the_asn1_tag a)
+  (* f2 *) (synth_the_asn1_tag a)
+  (* s1 *) (serialize_u8
+            `serialize_filter`
+            filter_the_asn1_tag a)
+  (* g1 *) (synth_the_asn1_tag_inverse a)
+  (* prf*) ()
+  (* in *) (a')
+
