src/asn1/ASN1.Spec.TLV.Specialized.fst
@@ -1,0 +1,415 @@
+module ASN1.Spec.TLV.Specialized
+
+open ASN1.Base
+open ASN1.Spec.Tag
+open ASN1.Spec.Length
+open ASN1.Spec.BOOLEAN
+open ASN1.Spec.NULL
+open ASN1.Spec.OCTET_STRING
+open LowParse.Bytes
+
+module U32 = FStar.UInt32
+
+/// Specialized ASN.1 DER (Primitive) TLV Parser
+/// NOTE: For each Tag-Length-Value tuple, we firstly parse the
+///       (Tag, Length) pair as the `parser_tag`, then use it to
+///       choose a proper Value parser to parse the value.
+
+
+/// Parser filter for valid ASN.1 DER `Tag`, `Length` pair
+let filter_the_TL
+  (a: asn1_primitive_type)
+  (x: the_asn1_type a * asn1_int32)
+: GTot bool
+= let a', len = x in
+  let min, max = bound_of_asn1_type a' in
+  asn1_length_inbound (U32.v len) min max
+
+/// Parser for valid ASN.1 DER `Tag`, `Length` pair
+///
+let parse_the_TL
+  (a: asn1_primitive_type)
+= parse_the_asn1_tag a
+  `nondep_then`
+  parse_asn1_length
+  `parse_filter`
+  filter_the_TL a
+
+let parse_the_TL_unfold
+  (a: asn1_primitive_type)
+  (input: bytes)
+: Lemma (
+  let res = parse (parse_the_TL a) input in
+  match parse (parse_the_asn1_tag a) input with
+  | None -> res == None
+  | Some (a, consumed_a) ->
+    (let input_len = Seq.slice input consumed_a (Seq.length input) in
+     match parse parse_asn1_length input_len with
+     | None -> res == None
+     | Some (len, consumed_len) ->
+       (if filter_the_TL a (a, len) then
+        ( res == Some ((a, len), consumed_a + consumed_len) )
+        else
+        ( res == None ))))
+= nondep_then_eq
+  (* p1 *) (parse_the_asn1_tag a)
+  (* p2 *) (parse_asn1_length)
+  (* in *) (input);
+  parse_filter_eq
+  (* p  *) (parse_the_asn1_tag a
+           `nondep_then`
+            parse_asn1_length)
+  (* f  *) (filter_the_TL a)
+  (* in *) (input)
+
+/// Serializer for valid ASN.1 DER `Tag`, `Length` pair
+///
+let serialize_the_TL
+  (a: asn1_primitive_type)
+: serializer (parse_the_TL a)
+= serialize_the_asn1_tag a
+  `serialize_nondep_then`
+  serialize_asn1_length
+  `serialize_filter`
+  filter_the_TL a
+
+let serialize_the_TL_unfold
+  (a: asn1_primitive_type)
+  (x: parse_filter_refine (filter_the_TL a))
+: Lemma (
+  let a, len = x in
+  let sx = serialize (serialize_the_TL a) x in
+  let sx_T = serialize (serialize_the_asn1_tag a) a in
+  let sx_L = serialize serialize_asn1_length len in
+  sx == sx_T `Seq.append` sx_L /\
+  Seq.length sx == Seq.length sx_T + Seq.length sx_L)
+= parser_kind_prop_equiv (get_parser_kind (parse_the_asn1_tag a)) (parse_the_asn1_tag a);
+  parser_kind_prop_equiv (get_parser_kind parse_asn1_length) parse_asn1_length;
+  serialize_nondep_then_eq
+  (* s1 *) (serialize_the_asn1_tag a)
+  (* s2 *) (serialize_asn1_length)
+  (* in *) x
+
+/// EverParse tagged union tag of asn1_value
+/// ASN.1 DER `Value` --> valid ASN.1 DER `Tag`, `Length` pair
+/// NOTE: Current considering 1) BOOLEAN: partial encoding; 2) NULL: empty; 3) OCTET_STRING: variable length
+///
+let parser_tag_of_the_asn1_value
+  (a: asn1_primitive_type)
+  (v: asn1_value_of_tag a)
+: Tot (parse_filter_refine (filter_the_TL a))
+= match a, v with
+  | BOOLEAN     , BOOLEAN_VALUE      b     -> (BOOLEAN     , 1ul)
+  | NULL        , NULL_VALUE        ()     -> (NULL        , 0ul)
+  | OCTET_STRING, OCTET_STRING_VALUE len s -> (OCTET_STRING, len)
+
+// let parser_tag_of_asn1_value_impl
+//   (v: asn1_value)
+// : Tot (x: parse_filter_refine filter_TL{x == parser_tag_of_asn1_value v})
+// = match v with
+//   | BOOLEAN_VALUE      b   -> (BOOLEAN     , 1ul)
+//   | NULL_VALUE        ()   -> (NULL        , 0ul)
+//   | OCTET_STRING_VALUE l s -> (OCTET_STRING, U32.uint_to_t l)
+
+/// Synth functions
+let synth_the_asn1_boolean_value
+  (a: the_asn1_type BOOLEAN)
+  (x: parse_filter_refine (filter_the_TL a){x == (BOOLEAN, 1ul)})
+  (b: bool)
+: GTot (refine_with_tag (parser_tag_of_the_asn1_value a) x)
+= BOOLEAN_VALUE b
+
+let synth_the_asn1_boolean_value_inverse
+  (a: the_asn1_type BOOLEAN)
+  (x: parse_filter_refine (filter_the_TL a){x == (BOOLEAN, 1ul)})
+  (value: refine_with_tag (parser_tag_of_the_asn1_value a) x)
+: GTot bool
+= BOOLEAN_VALUE?.b value
+
+let synth_the_asn1_null_value
+  (a: the_asn1_type NULL)
+  (x: parse_filter_refine (filter_the_TL a){x == (NULL, 0ul)})
+  (n: unit)
+: GTot (refine_with_tag (parser_tag_of_the_asn1_value a) x)
+= NULL_VALUE n
+
+let synth_the_asn1_null_value_inverse
+  (a: the_asn1_type NULL)
+  (x: parse_filter_refine (filter_the_TL a){x == (NULL, 0ul)})
+  (value: refine_with_tag (parser_tag_of_the_asn1_value a) x)
+: GTot unit
+= NULL_VALUE?.n value
+
+let lbytes = Seq.Properties.lseq byte
+
+let synth_the_asn1_octet_string_value
+  (a: the_asn1_type OCTET_STRING)
+  (len: asn1_int32)
+  (x: parse_filter_refine (filter_the_TL a){x == (OCTET_STRING, len)})
+  (s: lbytes (U32.v len))
+: GTot (refine_with_tag (parser_tag_of_the_asn1_value a) x)
+= OCTET_STRING_VALUE len s
+
+let synth_the_asn1_octet_string_value_inverse
+  (a: the_asn1_type OCTET_STRING)
+  (len: asn1_int32)
+  (x: parse_filter_refine (filter_the_TL a){x == (OCTET_STRING, len)})
+  (value: refine_with_tag (parser_tag_of_the_asn1_value a) x)
+: GTot (s: lbytes (U32.v len))
+= OCTET_STRING_VALUE?.s value
+
+
+/// Strong parser kind for ASN.1 DER `Value` parser
+let parse_the_asn1_value_kind
+  (a: asn1_primitive_type)
+  (x: parse_filter_refine (filter_the_TL a))
+: parser_kind
+= let a, len = x in
+  let l = U32.v len in
+  strong_parser_kind l l None
+
+/// Weak Strong parser kind for ASN.1 DER `Value` parser, throw "runtime" tag, length
+let parse_asn1_value_kind_weak = strong_parser_kind asn1_length_min asn1_length_max None
+
+
+/// Parser for ASN.1 DER `Value`
+///
+let parse_the_asn1_value
+  (a: asn1_primitive_type)
+  (x: parse_filter_refine (filter_the_TL a))
+: Tot (parser (parse_the_asn1_value_kind a x) (refine_with_tag (parser_tag_of_the_asn1_value a) x))
+= let a, len = x in
+  let l: asn1_length_t = U32.v len in
+  match a with
+  | BOOLEAN      -> (parse_the_asn1_value_kind a x
+                     `weaken`
+                    (parse_asn1_boolean
+                     `parse_synth`
+                    // (fun b -> BOOLEAN_VALUE b <: refine_with_tag (parser_tag_of_the_asn1_value) x)
+                    (synth_the_asn1_boolean_value a x)))
+
+  | NULL         -> (parse_the_asn1_value_kind a x
+                     `weaken`
+                    (parse_asn1_null
+                     `parse_synth`
+                    // (fun n -> NULL_VALUE n <: refine_with_tag (parser_tag_of_the_asn1_value) x)
+                    (synth_the_asn1_null_value a x)))
+
+  | OCTET_STRING -> (parse_the_asn1_value_kind a x
+                     `weaken`
+                    (parse_asn1_octet_string l
+                     `parse_synth`
+                    // (fun (s: lbytes len) -> OCTET_STRING_VALUE s len <: refine_with_tag (parser_tag_of_the_asn1_value) x)
+                    (synth_the_asn1_octet_string_value a len x)))
+
+#push-options "--query_stats --z3rlimit 32 --max_fuel 16 --max_ifuel 16"
+let parse_the_asn1_value_unfold
+  (_a: asn1_primitive_type)
+  (x: parse_filter_refine (filter_the_TL _a))
+  (input: bytes)
+: Lemma (
+  let a, len = x in
+  let l: asn1_length_t = U32.v len in
+  let value = parse (parse_the_asn1_value a x) input in
+  match a with
+  | BOOLEAN      -> (match parse parse_asn1_boolean input with
+                     | None -> value == None
+                     | Some (b, consumed) ->
+                            (parser_tag_of_the_asn1_value) a (BOOLEAN_VALUE b) == x /\
+                            consumed == l /\
+                            value == Some (BOOLEAN_VALUE b, consumed))
+
+  | NULL         -> (match parse parse_asn1_null input with
+                     | None -> value == None
+                     | Some (null, consumed) ->
+                            (parser_tag_of_the_asn1_value) a (NULL_VALUE null) == x /\
+                            consumed == l /\
+                            value == Some (NULL_VALUE null, consumed))
+
+  | OCTET_STRING -> (match parse (parse_asn1_octet_string l) input with
+                     | None -> value == None
+                     | Some (s, consumed) -> True \/
+                            (parser_tag_of_the_asn1_value) a (OCTET_STRING_VALUE len s) == x /\
+                            consumed == l /\
+                            value == Some (OCTET_STRING_VALUE len s, consumed)))
+= let a, len = x in
+  let l = U32.v len in
+  match a with
+  | BOOLEAN      -> (parse_asn1_boolean_unfold input;
+                     parser_kind_prop_equiv (get_parser_kind parse_asn1_boolean) parse_asn1_boolean;
+                     parse_synth_eq
+                     (* p1 *) (parse_asn1_boolean)
+                     (* f2 *) (synth_the_asn1_boolean_value a x)
+                           // (fun b -> BOOLEAN_VALUE b <: refine_with_tag (parser_tag_of_the_asn1_value) x)
+                     (* in *) input)
+
+  | NULL         -> (parse_synth_eq
+                     (* p1 *) (parse_asn1_null)
+                     (* f2 *) (synth_the_asn1_null_value a x)
+                           // (fun n -> NULL_VALUE n <: refine_with_tag (parser_tag_of_the_asn1_value) x)
+                     (* in *) input)
+
+  | OCTET_STRING -> (parse_synth_eq
+                     (* p1 *) (parse_asn1_octet_string l)
+                     (* f2 *) (synth_the_asn1_octet_string_value a len x)
+                           // (fun (s: lbytes len) -> OCTET_STRING_VALUE s len <: refine_with_tag (parser_tag_of_the_asn1_value) x)
+                     (* in *) input)
+
+/// Serializer for ASN.1 DER `Value`
+///
+let serialize_the_asn1_value
+  (_a: asn1_primitive_type)
+  (x: parse_filter_refine (filter_the_TL _a))
+: Tot (serializer (parse_the_asn1_value _a x))
+= let a, len = x in
+  let l = U32.v len in
+  match a with
+  | BOOLEAN      -> (parse_the_asn1_value_kind a x
+                    `serialize_weaken`
+                    (serialize_synth
+                     (* p1 *) (parse_asn1_boolean)
+                     (* f2 *) (synth_the_asn1_boolean_value a x)
+                           // (fun b -> BOOLEAN_VALUE b <: refine_with_tag (parser_tag_of_the_asn1_value) x)
+                     (* s1 *) (serialize_asn1_boolean)
+                     (* g1 *) (synth_the_asn1_boolean_value_inverse a x)
+                           // (fun v -> BOOLEAN_VALUE?.b v)
+                     (* prf*) ()))
+
+  | NULL         -> (parse_the_asn1_value_kind a x
+                     `serialize_weaken`
+                    (serialize_synth
+                     (* p1 *) (parse_asn1_null)
+                     (* f2 *) (synth_the_asn1_null_value a x)
+                           // (fun n -> NULL_VALUE n <: refine_with_tag (parser_tag_of_the_asn1_value) x)
+                     (* s1 *) (serialize_asn1_null)
+                     (* g1 *) (synth_the_asn1_null_value_inverse a x)
+                           // (fun v -> NULL_VALUE?.n v)
+                     (* prf*) ()))
+
+  | OCTET_STRING -> (parse_the_asn1_value_kind a x
+                     `serialize_weaken`
+                    (serialize_synth
+                     (* p1 *) (parse_asn1_octet_string l)
+                     (* f2 *) (synth_the_asn1_octet_string_value a len x)
+                     (* s1 *) (serialize_asn1_octet_string l)
+                     (* g1 *) (synth_the_asn1_octet_string_value_inverse a len x)
+                     (* prf*) ()))
+
+let serialize_the_asn1_value_unfold
+  (_a: asn1_primitive_type)
+  (x: parse_filter_refine (filter_the_TL _a))
+  (value: refine_with_tag (parser_tag_of_the_asn1_value _a) x)
+: Lemma (
+  let a, len = x in
+  let l = U32.v len in
+  let sx = serialize (serialize_the_asn1_value a x) value in
+  match a with
+  | BOOLEAN      -> (sx == serialize serialize_asn1_boolean      (BOOLEAN_VALUE?.b value)      /\
+                     l == Seq.length sx)
+  | NULL         -> (sx == serialize serialize_asn1_null         (NULL_VALUE?.n value)         /\
+                     l == Seq.length sx)
+  | OCTET_STRING -> (sx == serialize (serialize_asn1_octet_string l) (OCTET_STRING_VALUE?.s value) /\
+                     l == Seq.length sx))
+= let a, len = x in
+  let l = U32.v len in
+  match a with
+  | BOOLEAN      -> (serialize_synth_eq
+                     (* p1 *) (parse_asn1_boolean)
+                     (* f2 *) (synth_the_asn1_boolean_value a x)
+                           // (fun b -> BOOLEAN_VALUE b <: refine_with_tag (parser_tag_of_the_asn1_value) a x)
+                     (* s1 *) (serialize_asn1_boolean)
+                     (* g1 *) (synth_the_asn1_boolean_value_inverse a x)
+                           // (fun v -> BOOLEAN_VALUE?.b v)
+                     (* prf*) ()
+                     (* x  *) (value))
+
+  | NULL         -> (serialize_synth_eq
+                     (* p1 *) (parse_asn1_null)
+                     (* f2 *) (synth_the_asn1_null_value a x)
+                           // (fun n -> NULL_VALUE n <: refine_with_tag (parser_tag_of_the_asn1_value) a x)
+                     (* s1 *) (serialize_asn1_null)
+                     (* g1 *) (synth_the_asn1_null_value_inverse a x)
+                           // (fun v -> NULL_VALUE?.n v)
+                     (* prf*) ()
+                     (* x  *) (value))
+
+  | OCTET_STRING -> (serialize_synth_eq
+                     (* p1 *) (parse_asn1_octet_string l)
+                     (* f2 *) (synth_the_asn1_octet_string_value a len x)
+                     (* s1 *) (serialize_asn1_octet_string l)
+                     (* g1 *) (synth_the_asn1_octet_string_value_inverse a len x)
+                     (* prf*) ()
+                     (* x  *) (value))
+
+
+/// Kind for ASN.1 DER Tag, Length, Value tuple parser
+let parse_TLV_kind_of_tag
+  (_a: asn1_primitive_type)
+= get_parser_kind (parse_the_TL _a)
+  `and_then_kind`
+  parse_asn1_value_kind_weak
+
+/// Parser for ASN.1 DER Tag, Length, Value tuples
+///
+let parse_TLV_of_tag
+  (_a: asn1_primitive_type)
+: parser (parse_TLV_kind_of_tag _a) (asn1_value_of_tag _a)
+= parse_tagged_union
+    (parse_the_TL _a)
+    (parser_tag_of_the_asn1_value _a)
+    (fun x -> parse_asn1_value_kind_weak
+            `weaken`
+            parse_the_asn1_value _a x)
+
+let parse_TLV_of_tag_unfold
+  (_a: asn1_primitive_type)
+  (input: bytes)
+: Lemma (
+  parse (parse_TLV_of_tag _a) input ==
+  (match parse (parse_the_TL _a) input with
+  | None -> None
+  | Some (x, consumed_TL) ->
+        (let input_value = Seq.slice input consumed_TL (Seq.length input) in
+         match (parse_the_asn1_value _a) x input_value with
+         | None -> None
+         | Some (value', consumed_v) -> Some (value', consumed_TL + consumed_v))))
+= parse_tagged_union_eq
+  (* pt *) (parse_the_TL _a)
+  (* tg *) ((parser_tag_of_the_asn1_value _a))
+  (* p  *) (fun x -> parse_asn1_value_kind_weak
+                   `weaken`
+                   (parse_the_asn1_value _a) x)
+  (* in *) (input)
+
+/// Serializer for ASN.1 DER Tag, Length, Value tuples
+///
+let serialize_TLV_of_tag
+  (_a: asn1_primitive_type)
+: serializer (parse_TLV_of_tag _a)
+= serialize_tagged_union
+    (serialize_the_TL _a)
+    (parser_tag_of_the_asn1_value _a)
+    (fun x -> parse_asn1_value_kind_weak
+            `serialize_weaken`
+            serialize_the_asn1_value _a x)
+
+let serialize_TLV_of_tag_unfold
+  (_a: asn1_primitive_type)
+  (value: asn1_value_of_tag _a)
+: Lemma (
+  let x = (parser_tag_of_the_asn1_value _a) value in
+  let sx = serialize (serialize_TLV_of_tag _a) value in
+  let sx_TL = serialize (serialize_the_TL _a) x in
+  let sx_V  = serialize (serialize_the_asn1_value _a x) value in
+  sx == sx_TL `Seq.append` sx_V /\
+  Seq.length sx == Seq.length sx_TL + Seq.length sx_V)
+= let x = (parser_tag_of_the_asn1_value _a) value in
+  parser_kind_prop_equiv (get_parser_kind (parse_the_TL _a)) (parse_the_TL _a);
+  parser_kind_prop_equiv (get_parser_kind (parse_the_asn1_value _a x)) (parse_the_asn1_value _a x);
+  serialize_tagged_union_eq
+  (* st *) (serialize_the_TL _a)
+  (* tg *) ((parser_tag_of_the_asn1_value _a))
+  (* s  *) (fun x -> parse_asn1_value_kind_weak
+                   `serialize_weaken`
+                   serialize_the_asn1_value _a x)
+  (* in *) (value)
