src/asn1/ASN1.Spec.Tag.fsti
@@ -6,11 +6,13 @@ include LowParse.Spec.Int
 
 include ASN1.Base
 
+/// Generic
+///
 val filter_asn1_tag
   (b: byte)
 : Ghost bool
   (requires True)
-  (ensures fun r -> r == (b = 0x01uy || b = 0x04uy || b = 0x05uy))
+  (ensures fun r -> r == (b = 0x01uy || b = 0x04uy || b = 0x05uy || b = 0x30uy))
 
 let valid_asn1_tag_byte = parse_filter_refine filter_asn1_tag
 
@@ -22,7 +24,8 @@ val synth_asn1_tag
     a == (match b with
           | 0x01uy -> BOOLEAN
           | 0x04uy -> OCTET_STRING
-          | 0x05uy -> NULL))
+          | 0x05uy -> NULL
+          | 0x30uy -> SEQUENCE))
 
 val synth_asn1_tag_inverse
   (a: asn1_type)
@@ -55,3 +58,54 @@ val serialize_asn1_tag_unfold
   serialize serialize_asn1_tag a
   `Seq.equal`
   serialize serialize_u8 (synth_asn1_tag_inverse a))
+
+/// Specialied
+///
+val filter_the_asn1_tag
+  (a: asn1_type)
+  (b: byte)
+: Ghost bool
+  (requires True)
+  (ensures fun r -> (r <==> filter_asn1_tag b /\ synth_asn1_tag b == a))
+
+val synth_the_asn1_tag
+  (a: asn1_type)
+  (b: parse_filter_refine (filter_the_asn1_tag a))
+: Ghost (the_asn1_type a)
+  (requires True)
+  (ensures fun a' -> (a' == synth_asn1_tag b))
+
+val synth_the_asn1_tag_inverse
+  (a: asn1_type)
+  (a': the_asn1_type a)
+: Ghost (parse_filter_refine (filter_the_asn1_tag a))
+  (requires True)
+  (ensures fun b -> (b == synth_asn1_tag_inverse a'))
+
+val parse_the_asn1_tag
+  (a: asn1_type)
+: parser parse_asn1_tag_kind (the_asn1_type a)
+
+val parse_the_asn1_tag_unfold
+  (a: asn1_type)
+  (input: bytes)
+: Lemma (
+  parse (parse_the_asn1_tag a) input ==
+ (match parse parse_u8 input with
+  | Some (x, consumed) -> if filter_the_asn1_tag a x then
+                          ( Some (synth_the_asn1_tag a x, consumed) )
+                          else
+                          ( None )
+  | None -> None))
+
+val serialize_the_asn1_tag
+  (a: asn1_type)
+: serializer (parse_the_asn1_tag a)
+
+val serialize_the_asn1_tag_unfold
+  (a: asn1_type)
+  (a': the_asn1_type a)
+: Lemma (
+  serialize (serialize_the_asn1_tag a) a'
+  `Seq.equal`
+  serialize serialize_u8 (synth_the_asn1_tag_inverse a a'))
